\textbf{Euler functions}

\begin{tabular}{l|l|l}
    $\displaystyle B(a, b) = \int_0^1x^{a-1}(1-x)^{b-1}dx$ &
    $\displaystyle \Gamma(a) = \int_0^\infty x^{a-1}e^{-x}dx$ &
    $\displaystyle \Gamma(n) \sim (n-1)!$ \\
    $\displaystyle B(a, b) = B(b, a)$ &
    $\displaystyle \Gamma > 0$ &
    $\displaystyle B(a, b) = \frac{\Gamma(a)\Gamma(b)}{\Gamma(a+b)}$ \\
    $\displaystyle B(a, b) = \frac{b-1}{a+b-1}B(a, b-1)$ &
    $\displaystyle \Gamma(a+1) = a\Gamma(a)$ &
    $\displaystyle \Gamma(a)\Gamma(1-a) = \frac{\pi}{\sin{\pi a}}$ \\
    $\displaystyle B(a, 1-a) = \frac{\pi}{\sin{\pi a}}$ &
    $\displaystyle \Gamma(1) = 1$ &
    $\displaystyle \Gamma\left(\frac{1}{2}\right) = \sqrt{\pi}, \Gamma\left(n+\frac{1}{2}\right) = \Gamma\left(n-\frac{1}{2}\right)\ldots\sqrt{\pi}$ \\
    \hline
\end{tabular}